Modify instance syntax and add files to CoqProject

typeclass/Interfaces/assetmapping_spl_int.v
@@ -5,16 +5,26 @@ Require Export Coq.Lists.List.
 
 Class AssetMapping (A N m: Type): Type :=
 {
-  assetRef : set A -> set A -> Prop;
+  (*====================functions=======================*)
+  assetRef  : set A -> set A -> Prop;
   wfProduct : set A -> Prop;
-  aMR : m -> m -> Prop;
-  assetRefinementReflexivity : forall x: set A, assetRef x x;
-  assetRefinementTranstivity : forall x y z: set A, assetRef x y -> assetRef y z ->  assetRef x z;
-  as_dec : forall x y:A, {x = y} + {x <> y};
-  asRefCompositional :  forall (S1 : set A) (S2 : set A) (aSet : set A),
+  aMR       : m -> m -> Prop;
+
+  (*===========Axioms - Lemmas - Theorems====================*)
+  assetRefinementReflexivity : 
+    forall x: set A, assetRef x x;
+  assetRefinementTranstivity : 
+    forall x y z: set A, 
+      assetRef x y -> assetRef y z ->  assetRef x z;
+  as_dec                     : 
+      forall x y:A, {x = y} + {x <> y};
+  asRefCompositional         :  
+    forall (S1 : set A) (S2 : set A) (aSet : set A),
       (assetRef S1 S2) /\ wfProduct (set_union as_dec S1 aSet) 
         -> (wfProduct (set_union as_dec S2 aSet)) 
           /\ assetRef (set_union as_dec S1 aSet) 
              (set_union as_dec S2 aSet);
-  assetMappingRefinement: forall x y z: m, aMR x x /\ aMR x y -> aMR y z ->  aMR x z;
+  assetMappingRefinement: 
+    forall x y z: m, 
+      aMR x x /\ aMR x y -> aMR y z ->  aMR x z;
 }.
