typeclass/Instances/assetmapping_spl_inst.v
@@ -12,21 +12,30 @@ Import Maps.
 Import AssetMappingSPL.  
 
 
-Instance Ins_AssetMapping: AssetMapping Asset AssetName AM :=
+Program Instance Ins_AssetMapping: AssetMapping Asset AssetName AM :=
 {
   assetRef      := assetRef_func;
   wfProduct     := wfProduct_ind;
   aMR           := aMR_func;
 }.
-Proof.
+Next Obligation.
   {(*assetRefinementReflexivity*)
    apply assetRefinementReflexivity_axiom.
-} { (*assetRefinementTranstivity*)
-   apply assetRefinementTranstivity_axiom.
-} { (*as_dec*)
+} Qed.
+Next Obligation.
+ { (*assetRefinementTranstivity*)
+  generalize H H0. apply assetRefinementTranstivity_axiom.
+} Qed.
+Next Obligation.
+{ (*as_dec*)
    apply as_dec_axiom.
-} { (*asRefCompositional*)
-   apply asRefCompositional_axiom.
-} { (*assetMappingRefinement*)
-  apply assetMappingRefinement_axiom.
+} Qed.
+Next Obligation.
+ { (*asRefCompositional*)
+  admit. (*apply asRefCompositional_axiom.*)
+} Admitted.
+Next Obligation. { (*assetMappingRefinement*)
+  generalize H0. apply assetMappingRefinement_axiom. split.
+    + apply H. 
+    + apply H1.
 } Qed.
