typeclass/Interfaces/cktrans_spl_int.v
@@ -5,21 +5,28 @@ Require Export Coq.Lists.List.
 
 Class CKTrans (F A AM ck Conf: Type): Type :=
 {
+  (*====================functions=======================*)
   CKSem         : ck -> AM -> Conf -> set A;
   CKConf        : ck -> set Conf;
   equivalentCKs : ck -> ck -> Prop;
   weakerEqCK    : F -> ck -> ck -> Prop;
+
+  (*===========Axioms - Lemmas - Theorems====================*)
   eqCK:
     forall ck1: ck, equivalentCKs ck1 ck1 /\
-      (forall ck1 ck2: ck, equivalentCKs ck1 ck2 -> equivalentCKs ck2 ck1) /\
-         (forall ck1 ck2 ck3: ck, equivalentCKs ck1 ck2 /\ equivalentCKs ck2 ck3 -> equivalentCKs ck1 ck3);
+      (forall ck1 ck2: ck, equivalentCKs ck1 ck2 
+        -> equivalentCKs ck2 ck1) /\
+         (forall ck1 ck2 ck3: ck, equivalentCKs ck1 ck2
+           /\ equivalentCKs ck2 ck3 -> equivalentCKs ck1 ck3);
   weakerEqReflexive: 
-    forall (fm: F) (ck1: ck), weakerEqCK fm ck1 ck1;
+    forall (fm: F) (ck1: ck),
+      weakerEqCK fm ck1 ck1;
   weakerEqSymmetric:
     forall (fm: F) (ck1 ck2: ck),
         weakerEqCK fm ck1 ck2 -> weakerEqCK fm ck2 ck1;
   weakerEqTransitive:
      forall (fm: F) (ck1 ck2 ck3: ck),
-        weakerEqCK fm ck1 ck2 -> weakerEqCK fm ck2 ck3 -> weakerEqCK fm ck1 ck3
+        weakerEqCK fm ck1 ck2 -> weakerEqCK fm ck2 ck3 
+          -> weakerEqCK fm ck1 ck3
   
 }.
